improved interface for SepLogFold + port

MirrorCharge!/src/SepLogFold.v
@@ -19,6 +19,7 @@ Section seplog_fold.
   Variable RSym_sym : RSym (typD ts) sym.
 
   Variable T : Type.
+  Variable SL : typ.
 
   Record SepLogArgs : Type :=
   { do_atomic_app : expr sym -> list (expr sym) -> T
@@ -27,43 +28,50 @@ Section seplog_fold.
   ; do_star : T -> T -> T
   }.
 
-  Variable is_pure : expr sym -> bool.
-  Variable is_emp : sym -> bool.
-  Variable is_star : sym -> bool.
+  Record SepLogSpec : Type :=
+  { is_pure : expr sym -> bool
+  ; is_emp : sym -> bool
+  ; is_star : sym -> bool
+  }.
 
-  Record SepLogArgsOk (ST : typ) (sla : SepLogArgs) : Type :=
-  { R_t : expr sym -> T -> tenv typ -> tenv typ -> Prop
-  ; Hatomic_app
+  Variable sla : SepLogArgs.
+  Variable sls : SepLogSpec.
+
+  Record SepLogArgsOk (R_t : expr sym -> T -> tenv typ -> tenv typ -> Prop) : Type :=
+  { atomic_appOk
     : forall e es tus tvs,
-        typeof_apps _ tus tvs e es = Some ST ->
+        typeof_apps _ tus tvs e es = Some SL ->
         R_t (apps e es) (sla.(do_atomic_app) e es) tus tvs
-  ; Hpure
+  ; pureOk
     : forall e tus tvs,
-        typeof_expr tus tvs e = Some ST ->
-        is_pure e = true ->
+        typeof_expr tus tvs e = Some SL ->
+        sls.(is_pure) e = true ->
         R_t e (sla.(do_pure) e) tus tvs
-  ; Hemp
+  ; empOk
     : forall e tus tvs,
-        typeof_sym e = Some ST ->
-        is_emp e = true ->
+        typeof_sym e = Some SL ->
+        sls.(is_emp) e = true ->
         R_t (Inj e) sla.(do_emp) tus tvs
-  ; Hstar
+  ; starOk
     : forall e l r l_res r_res tus tvs,
-        typeof_sym e = Some (tyArr ST (tyArr ST ST)) ->
-        typeof_expr tus tvs l = Some ST ->
-        typeof_expr tus tvs r = Some ST ->
-        is_star e = true ->
+        typeof_sym e = Some (tyArr SL (tyArr SL SL)) ->
+        typeof_expr tus tvs l = Some SL ->
+        typeof_expr tus tvs r = Some SL ->
+        sls.(is_star) e = true ->
         R_t l l_res tus tvs ->
         R_t r r_res tus tvs ->
         R_t (apps (Inj e) (l :: r :: nil)) (sla.(do_star) l_res r_res) tus tvs
   }.
 
   Definition AppFullFoldArgs_SepLogArgs (sla : SepLogArgs) : AppFullFoldArgs sym T :=
-    match sla with
+    match sla , sls with
       | {| do_atomic_app := do_atomic_app
          ; do_pure := do_pure
          ; do_star := do_star
-         ; do_emp := do_emp |} =>
+         ; do_emp := do_emp |}
+      , {| is_pure := is_pure
+         ; is_star := is_star
+         ; is_emp := is_emp |} =>
         {| do_var := fun v _ _ => do_atomic_app (Var v) nil
          ; do_uvar := fun u _ _ => do_atomic_app (UVar u) nil
          ; do_inj := fun i _ _ =>
@@ -90,98 +98,90 @@ Section seplog_fold.
     end.
 
   Section sound.
-    Context SL sla `{slaok : SepLogArgsOk SL sla}.
+    Context R_t `{slaok : SepLogArgsOk R_t}.
 
     Lemma atomic_ok
     : forall (tus tvs : tenv typ) e (t : typ),
         typeof_expr tus tvs e = Some t ->
         t = SL ->
-        R_t slaok e (sla.(do_atomic_app) e nil) tus
-            tvs.
+        R_t e (sla.(do_atomic_app) e nil) tus tvs.
     Proof.
-      destruct sla; simpl; intros; subst.
+      destruct slaok. simpl; intros. subst.
       change e with (apps e nil) at 1.
-      eapply Hatomic_app. unfold typeof_apps.
+      eapply atomic_appOk0. unfold typeof_apps.
       simpl. rewrite H. auto.
     Qed.
 
     Hypothesis BILOps : BILOperators (typD ts nil SL).
     Hypothesis is_starOk
     : forall i,
-        is_star i = true ->
-        let starT := tyArr SL (tyArr SL SL) in
-        exists pf : typeof_sym i = Some starT,
-          sepSP = match pf in _ = u
-                        return match u with
-                                 | Some t => typD ts nil t
-                                 | None => unit
-                               end
-                  with
-                    | eq_refl => symD i
-                  end.
+        sls.(is_star) i = true ->
+        typeof_sym i = Some (tyArr SL (tyArr SL SL)).
 
     Definition AppFullFoldArgsOk_SepLogsOk
-    : AppFullFoldArgsOk _ (AppFullFoldArgs_SepLogArgs sla).
+    : AppFullFoldArgsOk _ (AppFullFoldArgs_SepLogArgs sla)
+                        (fun t e res tus tvs =>
+                           t = SL ->
+                           R_t e res tus tvs).
     Proof.
-      refine (
-          @Build_AppFullFoldArgsOk _ _ _ _ _
-                                   (fun t e res tus tvs =>
-                                      t = SL ->
-                                      slaok.(R_t) e res tus tvs)
-                                   _ _ _ _ _).
-      { destruct sla; simpl; intros; subst.
-        change (Var v) with (apps (@Var sym v) nil) at 1.
-        eapply Hatomic_app. unfold typeof_apps.
-        simpl; rewrite H; auto. }
-      { destruct sla; simpl; intros; subst.
-        change (UVar v) with (apps (@UVar sym v) nil) at 1.
-        eapply Hatomic_app. unfold typeof_apps.
-        simpl. rewrite H. auto. }
-      { destruct sla; simpl; intros; subst.
-        change (Inj v) with (apps (@Inj sym v) nil) at 1.
-        consider (is_emp v); intros.
-        { eapply Hemp; eauto. }
-        { eapply Hatomic_app. unfold typeof_apps.
-          simpl. rewrite H. auto. } }
-      { destruct sla; simpl; intros; subst.
-        change (Abs t e) with (apps (Abs t e) nil) at 1.
-        eapply Hatomic_app. unfold typeof_apps.
-        simpl. rewrite H. auto. }
-      { intros. subst ft. subst.
-        destruct sla; simpl.
+      remember sla as s; destruct s; simpl; remember sls as s; destruct s.
+      constructor.
+      { simpl; intros.
+        replace do_atomic_app0 with (sla.(do_atomic_app)).
+        eapply atomic_ok; eauto. rewrite <- Heqs; reflexivity. }
+      { simpl; intros.
+        replace do_atomic_app0 with (sla.(do_atomic_app)).
+        eapply atomic_ok; eauto. rewrite <- Heqs; reflexivity. }
+      { simpl; intros.
+        consider (is_emp0 v); intros.
+        { replace do_emp0 with (sla.(do_emp)).
+          eapply (@empOk _ slaok); eauto.
+          Cases.rewrite_all_goal. auto.
+          rewrite <- Heqs0. simpl. auto.
+          rewrite <- Heqs. reflexivity. }
+        { replace do_atomic_app0 with (sla.(do_atomic_app)).
+          eapply atomic_ok; eauto. rewrite <- Heqs; reflexivity. } }
+      { simpl; intros.
+        replace do_atomic_app0 with (sla.(do_atomic_app)).
+        eapply atomic_ok; eauto. rewrite <- Heqs; reflexivity. }
+      { intros. subst ft. simpl.
         assert (typeof_apps RSym_sym tus tvs l (map fst rs) = Some SL).
-        { rewrite <- typeof_expr_apps. auto. }
-        destruct l; try solve [ eapply Hatomic_app; eauto ].
-        consider (is_star s); intros.
-        { generalize H3. eapply is_starOk in H3. destruct H3.
-          unfold typeof_apps in H2.
-          simpl in H2. rewrite x in H2.
-          destruct rs; simpl in *.
-          { rewrite x in H. clear - H. inv_all.
-            symmetry in H. eapply tyArr_circ_L in H. intuition. }
-          { inversion H1; clear H1; subst.
-            inversion H8; clear H8; subst.
-            { subst. simpl in *. forward; inv_all; try subst.
-              exfalso. eapply tyArr_circ_L; eauto. }
-            { subst. inversion H4; clear H4; subst.
-              { forward. subst. simpl in *.
-                inv_all; subst.
-                intuition. inv_all; subst.
-                unfold type_of_apply in *.
-                rewrite x in *. rewrite H7 in *. rewrite H in *.
-                forward. inv_all. clear H13. revert H6 H10. subst.
-                intros.
-                eapply Hstar; eauto. }
-              { intuition. simpl in *.
-                rewrite typeof_expr_apps in H.
-                unfold typeof_apps in H. simpl in H.
-                rewrite H8 in *. rewrite H7 in *. rewrite H1 in *.
-                rewrite x in *.
-                unfold type_of_apply in *.
-                forward; inv_all; subst. inv_all; subst.
-                eapply type_of_applys_circle_False in H14. intuition. } } } }
-        { eapply Hatomic_app; eauto. } }
-    Defined.
+        { rewrite <- typeof_expr_apps. congruence. }
+        generalize (atomic_appOk slaok). rewrite <- Heqs. simpl.
+        destruct l; auto.
+        consider (is_star0 s); eauto; intros.
+        { generalize H4. eapply is_starOk in H4.
+          unfold typeof_apps in H3.
+          simpl in H3. rewrite H4 in *.
+          inversion H1; clear H1; try subst.
+          { subst rs ts0; intros.
+            simpl in *. clear - H3. inv_all.
+            symmetry in H3. eapply tyArr_circ_L in H3. intuition. }
+          { subst rs ts0. inversion H7; clear H7.
+            { subst l l'; intros; simpl in *.
+              rewrite H4 in *. forward.
+              intuition. inv_all. subst y t0.
+              clear - H8. symmetry in H8.
+              eapply tyArr_circ_L in H8. intuition. }
+            { subst l l'. inversion H8; clear H8.
+              { subst l0 l'0. intuition. subst t.
+                destruct y, y0; simpl in *.
+                rewrite H8 in *. rewrite H6 in *. rewrite H4 in *.
+                unfold type_of_apply in *. forward.
+                inv_all.
+                subst x0 x t1 t2 t3 p0 p.
+                replace do_star0 with (sla.(do_star));
+                  [ | rewrite <- Heqs; reflexivity ].
+                eapply (starOk slaok); eauto.
+                rewrite <- Heqs0. auto. }
+              { exfalso. clear Heqs Heqs0. subst.
+                simpl in H3. intuition.
+                rewrite H2 in *. rewrite H6 in *. rewrite H1 in *.
+                forward. inv_all; try subst.
+                clear H15 H13. subst x x0 x1.
+                clear - H14.
+                eapply type_of_applys_circle_False in H14. auto. } } } } }
+    Qed.
 
     Definition seplog_fold (sla : SepLogArgs) : expr sym -> tenv typ -> tenv typ -> T :=
       app_fold_args (AppFullFoldArgs_SepLogArgs sla).
@@ -190,12 +190,10 @@ Section seplog_fold.
     : forall e tus tvs result,
         seplog_fold sla e tus tvs = result ->
         typeof_expr tus tvs e = Some SL ->
-        slaok.(R_t) e result tus tvs.
+        R_t e result tus tvs.
     Proof.
       intros.
-      eapply app_fold_args_sound in H. 2: eapply H0.
-      revert H. instantiate (1 := AppFullFoldArgsOk_SepLogsOk).
-      simpl. intuition.
+      eapply (app_fold_args_sound AppFullFoldArgsOk_SepLogsOk) in H; eauto. 
     Qed.
   End sound.
 End seplog_fold.
