MirrorCharge!/src/ILFFold.v
@@ -191,7 +191,7 @@ Section fold.
         generalize dependent (App e1_1 e1_2). clear e1_1 e1_2.
         intros. unfold type_of_apply in *.
         forward; inv_all; subst.
-        assert (Forall2 (fun t x => 
+        assert (Forall2 (fun t x =>
                               typeof_expr tus tvs (fst x) = Some t
                            /\ R_t t (fst x) (snd x tus tvs) tus tvs)
                         (t1 :: nil)
